ex 7.10

Chap7_2.thy
@@ -12,21 +12,29 @@ datatype com = SKIP
   | While bexp com ("(WHILE _/ DO _)"  [0, 61] 61)
   | Repeat com bexp ("(REPEAT _/ UNTIL _)")
   | Choice com com ("_ OR _" [60, 61] 60)
+  | THROW
+  | TryCatch com com ("(TRY _/ CATCH _)")
 
 value "''x'' ::= Plus (V ''y'') (N 1) ;; ''y'' ::= N 2"
 
-inductive big_step :: "com \<times> state \<Rightarrow> state \<Rightarrow> bool" (infix "\<Rightarrow>" 55) where
-Skip: "(SKIP, s) \<Rightarrow> s"
-| Assign: "(x ::= a, s) \<Rightarrow> s(x := aval a s)"
-| Seq: "\<lbrakk> (c1, s1) \<Rightarrow> s2; (c2, s2) \<Rightarrow> s3 \<rbrakk> \<Longrightarrow> (c1 ;; c2, s1) \<Rightarrow> s3"
+inductive big_step :: "com \<times> state \<Rightarrow> com \<times> state \<Rightarrow> bool" (infix "\<Rightarrow>" 55) where
+Skip: "(SKIP, s) \<Rightarrow> (SKIP, s)"
+| Throw: "(THROW, s) \<Rightarrow> (THROW, s)"
+| Assign: "(x ::= a, s) \<Rightarrow> (SKIP, s(x := aval a s))"
+| Seq: "\<lbrakk> (c1, s1) \<Rightarrow> (SKIP, s2); (c2, s2) \<Rightarrow> s3 \<rbrakk> \<Longrightarrow> (c1 ;; c2, s1) \<Rightarrow> s3"
+| SeqThrow: "(c1, s1) \<Rightarrow> (THROW, s2) \<Longrightarrow> (c1;; c2, s1) \<Rightarrow> (THROW, s2)"
 | IfTrue: "\<lbrakk> bval b s; (c1, s) \<Rightarrow> t \<rbrakk> \<Longrightarrow> (IF b THEN c1 ELSE c2, s) \<Rightarrow> t"
 | IfFalse: "\<lbrakk> \<not>bval b s; (c2, s) \<Rightarrow> t \<rbrakk> \<Longrightarrow> (IF b THEN c1 ELSE c2, s) \<Rightarrow> t"
-| WhileTrue: "\<lbrakk> bval b s; (c, s) \<Rightarrow> t; (WHILE b DO c, t) \<Rightarrow> u \<rbrakk> \<Longrightarrow> (WHILE b DO c, s) \<Rightarrow> u"
-| WhileFalse: "\<not>bval b s \<Longrightarrow> (WHILE b DO c, s) \<Rightarrow> s"
-| RepeatTrue: "\<lbrakk> bval b t; (c, s) \<Rightarrow> t \<rbrakk> \<Longrightarrow> (REPEAT c UNTIL b, s) \<Rightarrow> t"
-| RepeatFalse: "\<lbrakk> \<not>bval b t; (c, s) \<Rightarrow> t; (REPEAT c UNTIL b, t) \<Rightarrow> u \<rbrakk> \<Longrightarrow> (REPEAT c UNTIL b, s) \<Rightarrow> u"
+| WhileTrue: "\<lbrakk> bval b s; (c, s) \<Rightarrow> (SKIP, t); (WHILE b DO c, t) \<Rightarrow> u \<rbrakk> \<Longrightarrow> (WHILE b DO c, s) \<Rightarrow> u"
+| WhileTrueThrow: "\<lbrakk> bval b s; (c, s) \<Rightarrow> (THROW, t) \<rbrakk> \<Longrightarrow> (WHILE b DO c, s) \<Rightarrow> (THROW, t)"
+| WhileFalse: "\<not>bval b s \<Longrightarrow> (WHILE b DO c, s) \<Rightarrow> (SKIP, s)"
+| RepeatTrue: "\<lbrakk> bval b t; (c, s) \<Rightarrow> (SKIP, t) \<rbrakk> \<Longrightarrow> (REPEAT c UNTIL b, s) \<Rightarrow> (SKIP, t)"
+| RepeatFalse: "\<lbrakk> \<not>bval b t; (c, s) \<Rightarrow> (SKIP, t); (REPEAT c UNTIL b, t) \<Rightarrow> u \<rbrakk> \<Longrightarrow> (REPEAT c UNTIL b, s) \<Rightarrow> u"
+| RepeatThrow: "\<lbrakk> (c, s) \<Rightarrow> (THROW, t) \<rbrakk> \<Longrightarrow> (REPEAT c UNTIL b, s) \<Rightarrow> (THROW, t)"
 | ChoiceLeft: "(c, s) \<Rightarrow> t \<Longrightarrow> (c OR c', s) \<Rightarrow> t"
 | ChoiceRight: "(c', s) \<Rightarrow> t \<Longrightarrow> (c OR c', s) \<Rightarrow> t"
+| Try: "(p, s) \<Rightarrow> (SKIP, s') \<Longrightarrow> (TRY p CATCH c, s) \<Rightarrow> (SKIP, s')"
+| Catch: "\<lbrakk> (c1, s1) \<Rightarrow> (THROW, s2); (c2, s2) \<Rightarrow> r' \<rbrakk> \<Longrightarrow> (TRY c1 CATCH c2, s1) \<Rightarrow> r'"
 
 schematic_goal ex: "(''x'' ::= N 5;; '' y'' ::= V ''x'', s) \<Rightarrow> ?t"
   apply (rule Seq)
@@ -40,10 +48,10 @@ thm ex[simplified]
 code_pred big_step .
 
 values "{t. (SKIP, \<lambda>_. 0) \<Rightarrow> t}"
-values "{map t [''x'', ''y''] | t. (''x'' ::= N 2, \<lambda>_. 0) \<Rightarrow> t}"
-values "{map t [''x''] |t. (SKIP, <''x'' := 42>) \<Rightarrow> t}"
-values "{map t [''x''] |t. (''x'' ::= N 2, <''x'' := 42>) \<Rightarrow> t}"
-values "{map t [''x'',''y''] |t.
+values "{map (snd t) [''x'', ''y''] | t. (''x'' ::= N 2, \<lambda>_. 0) \<Rightarrow> t}"
+values "{map (snd t) [''x''] |t. (SKIP, <''x'' := 42>) \<Rightarrow> t}"
+values "{map (snd t) [''x''] |t. (''x'' ::= N 2, <''x'' := 42>) \<Rightarrow> t}"
+values "{map (snd t) [''x'',''y''] |t.
   (WHILE Less (V ''x'') (V ''y'') DO (''x'' ::= Plus (V ''x'') (N 5)),
    <''x'' := 0, ''y'' := 13>) \<Rightarrow> t}"
 
@@ -54,6 +62,8 @@ lemmas big_step_induct = big_step.induct[split_format(complete)]
 
 inductive_cases SkipE[elim!]: "(SKIP, s) \<Rightarrow> t"
 thm SkipE
+inductive_cases ThrowE[elim!]: "(THROW, s) \<Rightarrow> t"
+thm ThrowE
 inductive_cases AssignE[elim!]: "(x ::= a, s) \<Rightarrow> t"
 thm AssignE
 inductive_cases SeqE[elim!]: "(c1 ;; c2, s1) \<Rightarrow> s3"
@@ -67,24 +77,16 @@ inductive_cases RepeatE[elim]: "(REPEAT c UNTIL b, s) \<Rightarrow> u"
 thm RepeatE
 inductive_cases ChoiceE[elim!]: "(p OR q, s) \<Rightarrow> t"
 thm ChoiceE
+inductive_cases TryCatchE[elim!]: "(TRY p CATCH c, s) \<Rightarrow> t"
+thm TryCatchE
 
 lemma assign_simp:
-"(x ::= a, s) \<Rightarrow> t \<longleftrightarrow> t = s(x := aval a s)"
+"(x ::= a, s) \<Rightarrow> (SKIP, t) \<longleftrightarrow> t = s(x := aval a s)"
   by blast
 
 lemma seq_assoc:
 "((c1;; c2);; c3, s) \<Rightarrow> t \<longleftrightarrow> (c1;; (c2;; c3), s) \<Rightarrow> t"
-proof
-  assume a1: "(c1;; c2;; c3, s) \<Rightarrow> t"
-  thm SeqE[OF a1]
-  obtain s1 where f1: "(c1 ;; c2, s) \<Rightarrow> s1" and f2: "(c3, s1) \<Rightarrow> t" by (elim SeqE[OF a1])
-  obtain s2 where f3: "(c1, s) \<Rightarrow> s2" and f4: "(c2, s2) \<Rightarrow> s1" by (elim SeqE[OF f1])
-  have f5: "(c2;; c3, s2) \<Rightarrow> t" by (intro Seq[OF f4 f2])
-  show "(c1;; (c2;; c3), s) \<Rightarrow> t" by (intro Seq[OF f3 f5])
-next
-  assume "(c1;; (c2;; c3), s) \<Rightarrow> t"
-  thus "(c1;; c2;; c3, s) \<Rightarrow> t" by blast
-qed
+  by blast
 
 abbreviation equiv_c :: "com \<Rightarrow> com \<Rightarrow> bool" (infix "\<sim>" 50) where
 "c \<sim> c' \<equiv> (\<forall>s t. (c, s) \<Rightarrow> t = (c', s) \<Rightarrow> t)"
@@ -94,10 +96,43 @@ lemma "WHILE b DO c \<sim> IF b THEN c;; WHILE b DO c ELSE SKIP"
 
 lemma "c \<sim> IF b THEN c ELSE c" by blast
 
-lemma sim_while_cong_aux: "(WHILE b DO c, s) \<Rightarrow> t \<Longrightarrow> c \<sim> c' \<Longrightarrow> (WHILE b DO c', s) \<Rightarrow> t"
-  by (induct "WHILE b DO c" s t rule: big_step_induct; auto)
+lemma sim_while_cong_aux: "(WHILE b DO c, s) \<Rightarrow> (r, s') \<Longrightarrow> c \<sim> c' \<Longrightarrow> (WHILE b DO c', s) \<Rightarrow> (r, s')"
+  by (induct "WHILE b DO c" s r s' rule: big_step_induct; auto)
 
 lemma sim_while_cong: "c \<sim> c' \<Longrightarrow> WHILE b DO c \<sim> WHILE b DO c'"
-  using sim_while_cong_aux by meson
+  using sim_while_cong_aux by (metis surj_pair)
+
+lemma sim_rep_cong_aux: "(REPEAT c UNTIL b, s) \<Rightarrow> (r, s') \<Longrightarrow> c \<sim> c' \<Longrightarrow> (REPEAT c' UNTIL b, s) \<Rightarrow> (r, s')"
+  by (induct "REPEAT c UNTIL b" s r s' rule: big_step_induct; auto)
+
+lemma sim_rep_cong: "c \<sim> c' \<Longrightarrow> (REPEAT c UNTIL b) \<sim> REPEAT c' UNTIL b"
+  using sim_rep_cong_aux by fastforce
+
+fun is_det :: "com \<Rightarrow> bool" where
+"is_det SKIP = True"
+| "is_det (x ::= a) = True"
+| "is_det (p ;; q) = (is_det p \<and> is_det q)"
+| "is_det (IF b THEN p ELSE q) = (is_det p \<and> is_det q)"
+| "is_det (WHILE b DO p) = is_det p"
+| "is_det (REPEAT p UNTIL b) = is_det p"
+| "is_det THROW = True"
+| "is_det (TRY p CATCH q) = (is_det p \<and> is_det q)"
+| "is_det (p OR q) = False"
+
+lemma big_step_det: "\<lbrakk> (p, s) \<Rightarrow> t; (p, s) \<Rightarrow> t'; is_det p \<rbrakk> \<Longrightarrow> t = t'"
+  apply (induct "(p, s)" t arbitrary: p s t' rule: big_step.induct)
+                  apply (blast+)[3]
+               apply (metis Pair_inject SeqE com.distinct(13) is_det.simps(3))
+  using is_det.simps(3) apply blast
+             apply (force, force)
+           apply (metis Pair_inject WhileE com.distinct(13) is_det.simps(5))
+          apply (metis WhileE com.distinct(13) is_det.simps(5) old.prod.inject)
+         apply blast
+        apply (metis (no_types, lifting) RepeatE is_det.simps(6) snd_conv)
+       apply (smt (verit, best) RepeatE com.distinct(13) is_det.simps(6) prod.inject)
+      apply (metis Pair_inject RepeatE com.simps(21) is_det.simps(6))
+     apply auto[2]
+  using is_det.simps(8) apply blast
+  by (metis Pair_inject TryCatchE com.distinct(13) is_det.simps(8))
 
 end
