Chap7ex.thy
@@ -10,8 +10,10 @@ fun assigned :: "com \<Rightarrow> vname set" where
 | "assigned (WHILE v DO va) = assigned va"
 | "assigned (REPEAT v UNTIL va) = assigned v"
 | "assigned (p OR q) = assigned p \<union> assigned q"
+| "assigned THROW = {}"
+| "assigned (TRY p CATCH c) = assigned p \<union> assigned c"
 
-lemma "\<lbrakk> (c, s) \<Rightarrow> t; x \<notin> assigned c \<rbrakk> \<Longrightarrow> s x = t x"
+lemma "\<lbrakk> (c, s) \<Rightarrow> (r, s'); x \<notin> assigned c \<rbrakk> \<Longrightarrow> s x = s' x"
   apply (induct rule: big_step_induct)
   by auto
 
@@ -23,26 +25,15 @@ fun skip :: "com \<Rightarrow> bool" where
 | "skip (WHILE v DO va) = (\<forall>s. \<not>bval v s)"
 | "skip (REPEAT v UNTIL va) = (skip v \<and> (\<forall>s. bval va s))"
 | "skip (p OR q) = (skip p \<and> skip q)"
+| "skip THROW = False"
+| "skip (TRY p CATCH c) = (skip p \<and> skip c)"
 
 lemma "skip c \<Longrightarrow> c \<sim> SKIP"
   apply (induct c rule: skip.induct; clarsimp)
   using assign_simp apply auto[1]
   apply fastforce
   apply (metis Chap7_2.IfE big_step.IfFalse big_step.IfTrue)
-  by auto
-
-lemma skip_while_aux: "\<lbrakk> (WHILE b DO c, s) \<Rightarrow> s'; bval b s \<rbrakk> \<Longrightarrow> \<not>bval b s'"
-  apply (induct "WHILE b DO c" s s' rule: big_step_induct)
   by blast+
-
-lemma skip_while: "bval b s \<Longrightarrow> \<not>(WHILE b DO c \<sim> SKIP)"
-text \<open>if the loop halts after n iterations, then @{term "(WHILE b DO c, s) \<Rightarrow> sn"} and since
-@{term "bval b s \<noteq> bval b sn"}, @{term "s \<noteq> sn"}. otherwise, the loop never halts,
-so for all t, @{term "(WHILE b DO c, s) \<Rightarrow> t"} does not hold.\<close>
-  using skip_while_aux by blast
-
-lemma "WHILE b DO c \<sim> SKIP = skip (WHILE b DO c)"
-  by (metis Chap7_2.SkipE Chap7_2.WhileE Skip WhileFalse skip.simps(5) skip_while_aux)
 
 lemma "x ::= (V x) \<sim> SKIP"
   using assign_simp by auto
@@ -59,8 +50,8 @@ IF (Bc True) THEN c1 ELSE c2 \<sim> SKIP"
 
 lemma "c \<sim> SKIP \<Longrightarrow> skip c"
   apply (induction c)
-      apply simp_all
-     apply (metis Chap7_2.SkipE big_step.Assign fun_upd_idem_iff)
+          apply simp_all
+         apply (metis Skip assign_simp fun_upd_idem_iff)
   oops
 
 fun skip' :: "com \<Rightarrow> bool" where
@@ -71,11 +62,14 @@ fun skip' :: "com \<Rightarrow> bool" where
 | "skip' (WHILE v DO va) = False"
 | "skip' (REPEAT v UNTIL va) = False"
 | "skip' (p OR q) = (skip' p \<and> skip' q)"
+| "skip' THROW = False"
+| "skip' (TRY p CATCH c) = (skip' p \<and> skip' c)"
 
 lemma "skip' c \<Longrightarrow> c \<sim> SKIP"
   apply (induct c rule: skip'.induct; clarsimp)
-    apply fastforce
-  apply (metis Chap7_2.IfE big_step.IfFalse big_step.IfTrue)
+     apply fastforce
+    apply (metis Chap7_2.IfE big_step.IfFalse big_step.IfTrue)
+   apply (metis Chap7_2.ChoiceE big_step.ChoiceRight)
   by blast
 
 fun deskip :: "com \<Rightarrow> com" where
@@ -89,6 +83,8 @@ if p' = SKIP then q' else if q' = SKIP then p' else p';;q')"
 | "deskip (WHILE b DO p) = WHILE b DO deskip p"
 | "deskip (REPEAT p UNTIL b) = REPEAT deskip p UNTIL b"
 | "deskip (p OR q) = deskip p OR deskip q"
+| "deskip THROW = THROW"
+| "deskip (TRY p CATCH c) = TRY (deskip p) CATCH (deskip c)"
 
 lemma "deskip (SKIP ;; WHILE b DO (x ::= a;; SKIP)) = WHILE b DO x ::= a"
   by simp
@@ -96,51 +92,63 @@ lemma "deskip (SKIP ;; WHILE b DO (x ::= a;; SKIP)) = WHILE b DO x ::= a"
 lemma "deskip ((SKIP;; SKIP);; (SKIP;; SKIP)) = SKIP"
   by simp
 
-lemma sim_rep_cong_aux: "(REPEAT c UNTIL b, s) \<Rightarrow> t \<Longrightarrow> c \<sim> c' \<Longrightarrow> (REPEAT c' UNTIL b, s) \<Rightarrow> t"
-  by (induct "REPEAT c UNTIL b" s t rule: big_step_induct; auto)
+lemma skipr[simp]: "(p;;SKIP, s) \<Rightarrow> cs = (p, s) \<Rightarrow> cs"
+  by (smt (verit, del_insts) Chap7_2.SeqE Chap7_2.SkipE Seq SeqThrow bs_ref_ss final_iff_SKIP old.prod.exhaust ss_ref_bs star.simps)
+
+lemma skipl[simp]: "(SKIP;;p, s) \<Rightarrow> cs = (p, s) \<Rightarrow> cs"
+  by blast
 
 lemma "deskip c \<sim> c"
   apply (induction c rule: deskip.induct; clarsimp)
-                      apply (blast+)[7]
-                      apply (case_tac "deskip (vb;; vc) = SKIP"; simp)
-                      apply (metis Chap7_2.SeqE Chap7_2.SkipE Seq Skip)
-                      apply (blast+)[5]
-                      apply (case_tac "deskip (v;; va) = SKIP"; simp)
-                      apply (metis Chap7_2.SeqE Chap7_2.SkipE Seq Skip)
+                      apply (smt (verit, del_insts) Chap7_2.SeqE Seq SeqThrow Skip final_iff_SKIP ss_eq_bs Chap7_2.SkipE)
                       apply blast
-                      apply (case_tac "deskip (vb;; vc) = SKIP"; case_tac "deskip (v;; va) = SKIP"; simp)
-                      apply (metis (full_types) Chap7_2.SeqE Chap7_2.SkipE Seq)
-                      apply ((metis Chap7_2.SeqE Chap7_2.SkipE Seq Skip)+)[2]
+                      apply auto[2]
                       apply blast
-                      apply ( case_tac "deskip (v;; va) = SKIP"; simp)
-                      apply (metis Chap7_2.SeqE Chap7_2.SkipE Seq Skip)
                       apply blast
-                      apply (case_tac "deskip (v;; va) = SKIP"; simp)
-                      apply (metis Chap7_2.SeqE Chap7_2.SkipE Seq Skip)
-                      apply (meson Chap7_2.SeqE Seq)
-                      apply (case_tac "deskip (v;; va) = SKIP"; simp)
-                      apply (metis Chap7_2.SeqE Chap7_2.SkipE Seq Skip)
+                      apply (smt (verit) Chap7_2.SeqE Chap7_2.SkipE Pair_inject Seq SeqThrow Skip com.distinct(13))
+                      apply (case_tac "deskip (vb;; vc) = SKIP"; case_tac "deskip (v;; va) = SKIP"; clarsimp)
+                      apply (smt (verit) Chap7_2.SeqE Chap7_2.SkipE Seq)
+                      apply (smt (verit, ccfv_threshold) Chap7_2.SeqE Chap7_2.SkipE Seq SeqThrow final_iff_SKIP ss_eq_bs star.simps)
+                      apply (smt (verit) Chap7_2.SeqE Chap7_2.SkipE Seq Skip com.distinct(13) old.prod.inject)
                       apply blast
-                      apply (case_tac "deskip (v;; va) = SKIP"; simp)
-                      apply (metis Chap7_2.SeqE Chap7_2.SkipE Seq Skip)
+                      apply (smt (verit) Chap7_2.SeqE Chap7_2.SkipE Pair_inject Seq SeqThrow Skip com.distinct(13))
+                      apply (smt (verit, ccfv_SIG) Chap7_2.SeqE Chap7_2.SkipE Seq SeqThrow Skip com.distinct(13) old.prod.inject)
+                      apply (smt (verit, ccfv_SIG) Chap7_2.SeqE Chap7_2.SkipE Pair_inject Seq SeqThrow Skip com.distinct(13))
+                      apply (smt (verit, del_insts) Chap7_2.SeqE Seq SeqThrow skipl)
+                      apply (smt (verit, best) Chap7_2.SeqE Chap7_2.SkipE Seq SeqThrow Skip prod.inject)
+                      apply (case_tac "deskip (v;; va) = SKIP"; clarsimp)
+                      apply (smt (verit, best) Chap7_2.SeqE Seq SeqThrow Skip skipl)
+                      apply (smt (verit, best) Chap7_2.SeqE Seq SeqThrow Skip skipl)
                       apply blast
-                      apply (meson Chap7_2.SeqE Seq)
-                      apply (case_tac "deskip (vc;; vd) = SKIP"; simp)
-                      apply (metis Chap7_2.SeqE Chap7_2.SkipE Seq Skip)
-                      apply ((meson Chap7_2.SeqE Seq)+)[6]
-                      apply (case_tac "deskip (vb;; vc) = SKIP"; simp)
-                      apply (metis Chap7_2.SeqE Chap7_2.SkipE Seq Skip)
-                      apply ((meson Chap7_2.SeqE Seq)+)[6]
-                apply (case_tac "deskip (vb;; vc) = SKIP"; simp)
-                 apply (metis Chap7_2.SeqE Chap7_2.SkipE Seq Skip)
-                apply ((meson Chap7_2.SeqE Seq)+)[6]
-          apply (case_tac "deskip (vb;; vc) = SKIP"; simp)
-           apply (metis Chap7_2.SeqE Chap7_2.SkipE Seq Skip)
-          apply ((meson Chap7_2.SeqE Seq)+)[6]
-      apply (blast+)[2]
-    apply (simp add: sim_while_cong)
-   apply (meson sim_rep_cong_aux)
-  by blast
+                      apply (smt (verit, ccfv_threshold) Chap7_2.SeqE Chap7_2.SkipE Seq SeqThrow Skip bs_ref_ss final_iff_SKIP)
+                      apply blast
+                      apply (smt (verit, ccfv_SIG) Chap7_2.SeqE Seq SeqThrow)
+  using SeqThrow apply (blast+)[4]
+                      apply auto[1]
+                      apply (smt (verit) Chap7_2.SeqE Chap7_2.SkipE Seq SeqThrow Skip final_iff_SKIP ss_eq_bs)
+                      apply (smt (verit, del_insts) Chap7_2.SeqE Seq SeqThrow)
+                      apply auto[2]
+                      apply (smt (verit) Chap7_2.SeqE Seq SeqThrow)
+                      apply auto[1]
+                      apply (smt (verit, ccfv_SIG) Chap7_2.SeqE Seq SeqThrow)
+                      apply auto[1]
+                      apply (smt (verit, ccfv_threshold) Chap7_2.SeqE Chap7_2.SkipE Seq SeqThrow Skip final_iff_SKIP ss_eq_bs)
+                      apply blast
+                      apply auto[2]
+  using SeqThrow apply (blast+)[4]
+                      apply (smt (verit, best) Chap7_2.SeqE Chap7_2.SkipE Seq SeqThrow Skip final_iff_SKIP ss_eq_bs)
+                      apply blast
+                      apply (smt (verit, ccfv_SIG) Chap7_2.SeqE Seq SeqThrow)
+  using Seq SeqThrow apply (blast+)[11]
+             apply (case_tac "deskip (vb;; vc) = SKIP"; clarsimp)
+              apply (smt (verit) Chap7_2.SeqE Seq SeqThrow skipr)
+             apply blast
+  using SeqThrow apply blast
+           apply (smt (verit, best) Chap7_2.SeqE Seq SeqThrow)
+  using SeqThrow apply (blast+)[5]
+  using sim_while_cong_aux apply fastforce
+  using sim_rep_cong_aux apply fastforce
+  by blast+
 
 inductive astep :: "aexp * state \<Rightarrow> aexp \<Rightarrow> bool" (infix "\<leadsto>" 50) where
 "(V x, s) \<leadsto> N (s x)"
@@ -173,43 +181,48 @@ lemma "IF And b1 b2 THEN c1 ELSE c2 \<sim> IF b1 THEN (IF b2 THEN c1 ELSE c2) EL
     by fastforce+
   done
 
-lemma helper_7_5: "\<not>(WHILE Bc True DO c, s) \<Rightarrow> t"
-  apply clarsimp
-  by (induct "WHILE Bc True DO c" s t rule: big_step_induct; simp)
-
 lemma "\<not>WHILE And b1 b2 DO c \<sim> WHILE b1 DO WHILE b2 DO c"
   if "b1 \<equiv> Eq (N 0) (V ''x'')" and "b2 \<equiv> Bc True" and "c \<equiv> ''x'' ::= Plus (V ''x'') (N 1)"
-and "s \<equiv> (\<lambda>_. 0) :: char list \<Rightarrow> int" and "t \<equiv> <''x'' := 1::int>"
+and "s \<equiv> <> :: (char list \<Rightarrow> int)" and "t \<equiv> <''x'' := 1::int>"
   apply clarsimp
   apply (rule exI[where x=s])
+  apply (rule exI[where x=SKIP])
   apply (rule exI[where x=t])
-  apply (subgoal_tac "(WHILE And b1 b2 DO c, s) \<Rightarrow> t")
-   apply (subgoal_tac "\<not> (WHILE b1 DO WHILE b2 DO c, s) \<Rightarrow> t")
-    apply simp
+  apply (subgoal_tac "(WHILE And b1 b2 DO c, s) \<Rightarrow> (SKIP, t)" "(WHILE b1 DO WHILE b2 DO c, s) \<Rightarrow> (SKIP, t) \<Longrightarrow> False")
+  apply blast
    apply (thin_tac "_")
-   apply clarsimp
    apply (erule Chap7_2.WhileE)
-  defer
-  unfolding that apply simp
-   apply (rule WhileTrue[where t=t])
-     apply simp
-    apply (subgoal_tac "t = (\<lambda>_. 0)(''x'' := 1)")
-  apply (simp add: assign_simp)
-  unfolding that(5)
-    apply (simp add: null_state_def)
-   apply (rule WhileFalse; simp)
-  using helper_7_5 by blast
+     apply (thin_tac "_")
+     apply (thin_tac "_ \<Rightarrow> (SKIP, t)")
+  subgoal for t
+    apply (induct "WHILE b2 DO c" s SKIP t rule: big_step_induct)
+    unfolding that(2) by auto
+  apply simp
+   apply (simp add: fun_upd_idem_iff null_state_def that(4) that(5))
+  apply (rule WhileTrue[where t=t])
+    apply (simp add: null_state_def that(1) that(2) that(4))
+  apply (subgoal_tac "t = s(''x'' := aval (Plus (V ''x'') (N 1)) s)")
+  using that(3) apply blast
+  apply (simp add: null_state_def that(4) that(5))
+  apply (rule WhileFalse)
+  by (simp add: that(1) that(5))
 
 abbreviation Or where "Or b1 b2 \<equiv> Not (And (Not b1) (Not b2))"
 
 lemma "WHILE Or b1 b2 DO c \<sim> WHILE Or b1 b2 DO c;; WHILE b1 DO c"
   apply clarsimp
-  subgoal for s t
-  apply (rule iffI)
-     apply (induct "WHILE Or b1 b2 DO c" s t rule: big_step_induct; clarsimp)
-      apply (metis Seq WhileTrue bval.simps(2) bval.simps(3))
-    apply (metis Seq WhileFalse bval.simps(2) bval.simps(3))
-    by (metis Chap7_2.SeqE Chap7_2.WhileE bval.simps(2) bval.simps(3) skip_while_aux)
+  subgoal for s t b
+    apply (rule iffI)
+     apply (induct "WHILE Or b1 b2 DO c" s t b rule: big_step_induct; clarsimp)
+       apply (smt (verit, ccfv_SIG) Chap7_2.SeqE Seq SeqThrow WhileTrue bval.simps(2) bval.simps(3))
+      apply (simp add: SeqThrow WhileTrueThrow)
+     apply (metis Seq WhileFalse bval.simps(2) bval.simps(3))
+    apply (erule Chap7_2.SeqE)
+    subgoal for s2
+      apply (induct "WHILE Or b1 b2 DO c" s SKIP s2 rule: big_step_induct; clarsimp)
+      using WhileTrue bval.simps(2) bval.simps(3) apply presburger
+      using WhileFalse by auto
+    by simp
   done
 
 definition DoWhile :: "com \<Rightarrow> bexp \<Rightarrow> com" ("(DO _ WHILE _)")where
@@ -220,12 +233,30 @@ fun dewhile :: "com \<Rightarrow> com" where
 | "dewhile (x ::= a) = x ::= a"
 | "dewhile (p ;; q) = dewhile p ;; dewhile q"
 | "dewhile (IF b THEN p ELSE q) = IF b THEN (dewhile p) ELSE (dewhile q)"
-| "dewhile (WHILE b DO c) = IF (Not b) THEN SKIP ELSE DO c WHILE b"
+| "dewhile (WHILE b DO c) = IF (Not b) THEN SKIP ELSE DO (dewhile c) WHILE b"
 | "dewhile (REPEAT c UNTIL b) = REPEAT dewhile c UNTIL b"
 | "dewhile (p OR q) = dewhile p OR dewhile q"
+| "dewhile THROW = THROW"
+| "dewhile (TRY p CATCH c) = TRY (dewhile p) CATCH (dewhile c)"
 
 lemma "dewhile c \<sim> c"
-  apply (induct c)
-  using DoWhile_def Seq Skip big_step.IfFalse big_step.IfTrue sim_rep_cong_aux by auto
+  apply (induct c; clarsimp)
+       apply blast
+      apply blast
+  subgoal for b c s r t
+    apply (rule iffI)
+     apply (erule Chap7_2.IfE)
+      apply auto[1]
+    unfolding DoWhile_def apply (erule Chap7_2.SeqE)
+      apply (simp add: WhileTrue sim_while_cong_aux)
+     apply (simp add: WhileTrueThrow)
+    apply (erule Chap7_2.WhileE)
+      apply (rule Chap7_2.IfFalse)
+    using bval.simps(2) apply blast
+      apply (simp add: Seq sim_while_cong_aux)
+     apply (simp add: SeqThrow big_step.IfFalse)
+    by (simp add: Skip big_step.IfTrue)
+    apply (simp add: sim_rep_cong)
+  by blast+
 
 end
